commit

AP/Game/Defs.lean
@@ -9,11 +9,21 @@ structure GameParams : Type (u + 1) where
   PState : Player → Type u
   PMove : Player → Player → Type u
   Outcome : Type u
-  
+
   h_inh_move : ∀ p, Inhabited # Move p
+  h_pl_fin : Fintype Player  
   h_pl_lin : LinearOrder Player
   h_out_lin : LinearOrder Outcome
   h_move_rfl : ∀ p, PMove p p = Move p
+
+instance {T : GameParams} : Fintype T.Player :=
+  T.h_pl_fin
+
+instance {T : GameParams} : LinearOrder T.Player :=
+  T.h_pl_lin
+
+instance {T : GameParams} : LinearOrder T.Outcome :=
+  T.h_out_lin
 
 def GameParams.Trans (T : GameParams) : Type u :=
   Σ (p : T.Player), T.Move p
@@ -21,59 +31,66 @@ def GameParams.Trans (T : GameParams) : Type u :=
 def GameParams.PTrans (T : GameParams) (p : T.Player) : Type u :=
   Σ (p' : T.Player), T.PMove p p'
 
-def GameParams.Rules (T : GameParams) : Type u :=
+def GameParams.GRules (T : GameParams) : Type u :=
   (p : T.Player) → T.State → T.Move p → Option (T.Player × T.State)
+
+abbrev GameParams.Hist (T : GameParams) : Type u :=
+  DMap T.Player # λ p => List (T.PTrans p)
 
 @[ext]
 structure GameParams.GState (T : GameParams) : Type u where
   player : T.Player
   state : T.State
-  hist : List T.Trans
+  hist : T.Hist
 
 def GameParams.initState (T : GameParams)
 (p : T.Player) (s : T.State) : T.GState :=
   { player := p
   , state := s
-  , hist := []
+  , hist := DMap.range # λ _ => []
   }
 
-def GameParams.sys_tr (T : GameParams) (rules : T.Rules)
-(s : T.GState) (t : T.Trans) : Option T.GState := by
-  haveI := T.h_pl_lin
-  exact if h : s.player ≠ t.1 then none else do
-  let (p₁, s₁) ← rules t.1 s.state t.2
-  some #
-    { player := p₁
-    , state := s₁
-    , hist := t :: s.hist
-    }
+def GameParams.GPMove (T : GameParams) : Type u :=
+  (p : T.Player) → T.GState → T.Trans → T.PTrans p
+
+def GameParams.updateHist (T : GameParams) (pmove : T.GPMove)
+(s : T.GState) (t : T.Move s.player) : T.Hist :=
+  s.hist.map # @λ p ts => pmove p s ⟨s.player, t⟩ :: ts
+
+def GameParams.sys_tr (T : GameParams) (rules : T.GRules) (pmove : T.GPMove)
+(s : T.GState) (t : T.Trans) : Option T.GState :=
+  if h : s.player = t.1 then do
+    let (p₁, s₁) ← rules t.1 s.state t.2
+    some #
+      { player := p₁
+      , state := s₁
+      , hist := T.updateHist pmove s # h ▸ t.2
+      }
+  else none
 
 @[ext]
 structure Game (T : GameParams) : Type u where
   sys : System T.GState T.Trans
   
-  rules : T.Rules
+  rules : T.GRules
   pstate : (p : T.Player) → T.State → T.PState p
-  pmove : (p : T.Player) → T.GState → (t : T.Trans) → List T.Trans → T.PTrans p
+  pmove : T.GPMove
   outcome : T.GState ⊕ (ℕ → T.GState) → T.Player → T.Outcome
   
-  h_sys_initial : sys.initial ≠ ∅
-  h_sys_tr : sys.tr = T.sys_tr rules
+  h_sys_init_nemp : sys.initial ≠ ∅
+  h_sys_init_valid : ∀ s ∈ sys.initial, ∃ p s', s = T.initState p s'
+  h_sys_tr : sys.tr = T.sys_tr rules pmove
 
 namespace Game
 
 variable {T : GameParams.{u}} (game : Game T)
 
-def getPMoves' (game : Game T) (s₀ : T.GState) (p : T.Player)
-(acc : List (T.PTrans p)) : List T.Trans → List (T.PTrans p)
-| [] => acc
-| (t :: ts) => game.getPMoves' s₀ p (game.pmove p s₀ t ts :: acc) ts
-
-def getPMoves (s₀ : T.GState) (p : T.Player)
-(ts : List T.Trans) : List (T.PTrans p) :=
-  (game.getPMoves' s₀ p [] ts).reverse
+def updateHist (s : T.GState) (t : T.Trans) : T.Hist :=
+  if h : s.player = t.1
+  then T.updateHist game.pmove s # h ▸ t.2
+  else s.hist
 
 structure Strat (s₀ : T.GState) (p : T.Player) : Type u where
   f : T.PState p → List (T.PTrans p) → T.Move p
   h : ∀ (s : T.GState), s.player = p → game.sys.has_tr s → game.sys.valid_tr s
-    ⟨p, f (game.pstate p s.state) (game.getPMoves s₀ p s.hist)⟩
+    ⟨p, f (game.pstate p s.state) (s.hist.get! p)⟩
