AP/Map/Basic.lean
@@ -1,29 +1,25 @@
 import AP.Map.Defs
 
-namespace Map
-
-set_option linter.unusedVariables false
 universe u
-variable {ι α : Type u} [hhι : LinearOrder ι] [hhα : DecidableEq α] {mp : Map ι α}
-set_option linter.unusedSectionVars true
+variable {ι : Type u} {α β : ι → Type u} [hhι : LinearOrder ι] {mp : DMap ι α}
 
-omit hhα in
-@[simp]
-theorem insert'_nil {x : ι × α} : insert' x [] = [x] := rfl
+namespace DMap
 
-omit hhα in
 @[simp]
-theorem insert'_cons {x y : ι × α} {xs : List (ι × α)} :
+theorem insert'_nil {x : Σ i, α i} : insert' x [] = [x] := rfl
+
+@[simp]
+theorem insert'_cons {x y : Σ i, α i} {xs : List (Σ i, α i)} :
 insert' x (y :: xs) = (match compare x.1 y.1 with
 | .eq => x :: xs
 | .lt => x :: y :: xs
 | .gt => y :: insert' x xs) := rfl
 
-theorem listCnd_of_cons {x : ι × α} {xs}
+theorem listCnd_of_cons {x : Σ i, α i} {xs}
 (h : listCnd (x :: xs)) : listCnd xs := by
   cases xs; trivial; exact h.2
 
-theorem listCnd_cons_of_le {x y : ι × α} {xs}
+theorem listCnd_cons_of_le {x y : Σ i, α i} {xs}
 (h₁ : listCnd (x :: xs)) (h₂ : y.1 ≤ x.1) : listCnd (y :: xs) := by
   cases xs
   · simp
@@ -33,17 +29,17 @@ theorem listCnd_cons_of_le {x y : ι × α} {xs}
   simp [h₃]
   exact lt_of_le_of_lt h₂ h₁
 
-theorem listCnd_cons_of_eq {x y : ι × α} {xs}
+theorem listCnd_cons_of_eq {x y : Σ i, α i} {xs}
 (h₁ : listCnd (x :: xs)) (h₂ : y.1 = x.1) : listCnd (y :: xs) := by
   apply listCnd_cons_of_le h₁; rw [h₂]
 
-theorem listCnd_cons_of_lt {x y : ι × α} {xs}
+theorem listCnd_cons_of_lt {x y : Σ i, α i} {xs}
 (h₁ : listCnd (x :: xs)) (h₂ : y.1 < x.1) : listCnd (y :: xs) := by
   apply listCnd_cons_of_le h₁; exact le_of_lt h₂
 
-theorem listCnd_map_of {β : Type u} [hb : DecidableEq β] (f : α → β)
-{xs : List (ι × α)} (h : listCnd xs) :
-listCnd # xs.map # λ x => (x.1, f x.2) := by
+theorem listCnd_map_of (f : ∀ {i}, α i → β i)
+{xs : List (Σ i, α i)} (h : listCnd xs) :
+listCnd # xs.map # λ x => ⟨x.1, f x.2⟩ := by
   induction xs
   · simp
   nm x xs ih
@@ -53,7 +49,7 @@ listCnd # xs.map # λ x => (x.1, f x.2) := by
   simp at h ih
   use h.1
 
-theorem listCnd_insert'_of {xs : List (ι × α)} {x}
+theorem listCnd_insert'_of {xs : List (Σ i, α i)} {x}
 (h : listCnd xs) : listCnd (insert' x xs) := by
   rcases x with ⟨i, x⟩
   generalize hn : xs.length = n
@@ -76,7 +72,7 @@ theorem listCnd_insert'_of {xs : List (ι × α)} {x}
   have h₂ := ih (n - 1)
   rw [←hn] at h₂
   specialize @h₂ (by simp) xs (listCnd_of_cons h) i x (by simp)
-  generalize hy : insert' (i, x) xs = ys at h₂ ⊢
+  generalize hy : insert' ⟨i, x⟩ xs = ys at h₂ ⊢
   cases ys
   · simp
   nm z ys
@@ -95,17 +91,17 @@ theorem listCnd_insert'_of {xs : List (ι × α)} {x}
     exact h₁
   exact h.1
 
-def insert_prod (x : ι × α) (mp : Map ι α) : Map ι α :=
+def insertProd (x : Σ i, α i) (mp : DMap ι α) : DMap ι α :=
   ⟨_, listCnd_insert'_of (x := x) mp.h⟩
 
-instance : Insert (ι × α) (Map ι α) :=
-  ⟨λ p mp => mp.insert_prod p⟩
+instance : Insert (Σ i, α i) (DMap ι α) :=
+  ⟨λ p mp => mp.insertProd p⟩
 
 @[simp]
-def insert (i : ι) (x : α) (mp : Map ι α) : Map ι α :=
-  mp.insert_prod (i, x)
+def insert (i : ι) (x : α i) (mp : DMap ι α) : DMap ι α :=
+  mp.insertProd ⟨i, x⟩
 
-theorem listCnd_ofList'_of {xs ys : List (ι × α)}
+theorem listCnd_ofList'_of {xs ys : List (Σ i, α i)}
 (h : listCnd xs) : listCnd (ofList' xs ys) := by
   induction ys generalizing xs
   · simpa
@@ -113,20 +109,27 @@ theorem listCnd_ofList'_of {xs ys : List (ι × α)}
   exact ih # listCnd_insert'_of h
 
 @[simp]
-theorem listCnd_ofList'_of_fst_nil {xs : List (ι × α)} :
+theorem listCnd_ofList'_of_fst_nil {xs : List (Σ i, α i)} :
 listCnd (ofList' [] xs) := by
   apply listCnd_ofList'_of; simp
 
-def ofList (xs : List (ι × α)) : Map ι α :=
+def ofList (xs : List (Σ i, α i)) : DMap ι α :=
   ⟨_, listCnd_ofList'_of_fst_nil (xs := xs)⟩
 
-def get? (i : ι) (mp : Map ι α) : Option α :=
-  lookup' i mp.toList
+def get? (i : ι) (mp : DMap ι α) : Option (α i) :=
+  get' i mp.toList
 
-def get! [Inhabited α] (i : ι) (mp : Map ι α) : α :=
+def get! (i : ι) [h : Inhabited (α i)] (mp : DMap ι α) : α i :=
   (mp.get? i).get!
 
-theorem lt_of_listCnd_cons_and_mem {xs : List (ι × α)} {x y}
+end DMap namespace Map
+
+def ofList {α : Type u} (xs : List (ι × α)) : Map ι α :=
+  DMap.ofList # xs.map # λ ⟨i, x⟩ => ⟨i, x⟩
+
+end Map namespace DMap
+
+theorem lt_of_listCnd_cons_and_mem {xs : List (Σ i, α i)} {x y}
 (h₁ : listCnd (x :: xs)) (h₂ : y ∈ xs) : x.1 < y.1 := by
   generalize hn : xs.length = n
   induction n using Nat.strong_induction_on generalizing x y xs
@@ -144,7 +147,7 @@ theorem lt_of_listCnd_cons_and_mem {xs : List (ι × α)} {x y}
   apply @ih (by simp) xs x y _ h₂ (by simp)
   exact listCnd_cons_of_lt h₃ h₁
 
-theorem listCnd_cons_of_forall_le {xs : List (ι × α)} {x}
+theorem listCnd_cons_of_forall_le {xs : List (Σ i, α i)} {x}
 (h₁ : listCnd xs) (h₂ : ∀ y ∈ xs, x.1 < y.1) : listCnd (x :: xs) := by
   cases xs
   · simp
@@ -154,13 +157,13 @@ theorem listCnd_cons_of_forall_le {xs : List (ι × α)} {x}
   simp at h₂
   exact h₂
 
-theorem listCnd_cons_iff {xs : List (ι × α)} {x} :
+theorem listCnd_cons_iff {xs : List (Σ i, α i)} {x} :
 listCnd (x :: xs) ↔ listCnd xs ∧ ∀ y ∈ xs, x.1 < y.1 := by
   use λ h => ⟨listCnd_of_cons h, λ _ => lt_of_listCnd_cons_and_mem h⟩
   use λ h => listCnd_cons_of_forall_le h.1 h.2
 
-theorem sorted_of_listCnd {xs : List (ι × α)}
-(h : listCnd xs) : xs.Sorted # λ (x y : ι × α) => x.1 < y.1 := by
+theorem sorted_of_listCnd {xs : List (Σ i, α i)}
+(h : listCnd xs) : xs.Sorted # λ (x y : Σ i, α i) => x.1 < y.1 := by
   induction xs
   · simp
   nm x xs ih
@@ -170,8 +173,8 @@ theorem sorted_of_listCnd {xs : List (ι × α)}
   intro y hy
   exact lt_of_listCnd_cons_and_mem h hy
 
-theorem listCnd_of_sorted {xs : List (ι × α)}
-(h : xs.Sorted # λ (x y : ι × α) => x.1 < y.1) : listCnd xs := by
+theorem listCnd_of_sorted {xs : List (Σ i, α i)}
+(h : xs.Sorted # λ (x y : Σ i, α i) => x.1 < y.1) : listCnd xs := by
   induction xs
   · simp
   nm x xs ih
@@ -181,11 +184,11 @@ theorem listCnd_of_sorted {xs : List (ι × α)}
   rw [listCnd_cons_iff]
   use ih
 
-theorem listCnd_iff_sorted {xs : List (ι × α)} :
-listCnd xs ↔ xs.Sorted (λ (x y : ι × α) => x.1 < y.1) :=
+theorem listCnd_iff_sorted {xs : List (Σ i, α i)} :
+listCnd xs ↔ xs.Sorted (λ (x y : Σ i, α i) => x.1 < y.1) :=
   ⟨sorted_of_listCnd, listCnd_of_sorted⟩
 
-theorem nodup_of_listCnd {xs : List (ι × α)} (h : listCnd xs) : xs.Nodup := by
+theorem nodup_of_listCnd {xs : List (Σ i, α i)} (h : listCnd xs) : xs.Nodup := by
   induction xs
   · simp
   nm x xs ih
@@ -196,3 +199,119 @@ theorem nodup_of_listCnd {xs : List (ι × α)} (h : listCnd xs) : xs.Nodup := b
   intro hx
   specialize h x hx
   simp at h
+
+def map (f : ∀ {i}, α i → β i) : DMap ι β := by
+  use mp.toList.map # λ ⟨i, x⟩ => ⟨i, f x⟩
+  apply listCnd_map_of
+  exact mp.h
+
+def range [fin : Fintype ι] (f : (i : ι) → α i) : DMap ι α :=
+  ofList # fin.1.to_sorted_list.map # λ i => ⟨i, f i⟩
+
+def mem (mp : DMap ι α) (i : ι) : Prop :=
+  mem' i mp.toList
+
+instance : Membership ι (DMap ι α) := ⟨mem⟩
+
+theorem mem_def {i : ι} : i ∈ mp ↔ mem' i mp.toList := by rfl
+
+theorem mem_iff_get?_eq_some {i : ι} : i ∈ mp ↔ ∃ x, mp.get? i = some x := by
+  rcases mp with ⟨xs, h₁⟩
+  simp [mem_def]
+  simp [get?]; clear h₁
+  induction xs <;> simp
+  nm x xs ih
+  split_ifs with h₁ <;> simp [h₁]
+  exact ih
+
+theorem get?_eq_some_of_mem {i : ι} (h : i ∈ mp) : ∃ x, mp.get? i = some x := by
+  rwa [←mem_iff_get?_eq_some]
+
+theorem get?_eq_none_of_not_mem {i : ι} (h : i ∉ mp) : mp.get? i = none := by
+  simp [mem_iff_get?_eq_some] at h
+  rwa [Option.eq_none_iff_forall_ne_some]
+
+theorem get?_map_eq {f : ∀ {i}, α i → β i} {i : ι} :
+(mp.map f).get? i = (mp.get? i).map f := by
+  rcases mp with ⟨xs, h⟩
+  simp [get?, map]
+  clear h
+  induction xs
+  · rfl
+  nm x xs ih
+  simp
+  split_ifs with h₁
+  · subst h₁
+    simp
+  exact ih
+
+theorem get!_map_eq_of_pos {f : ∀ {i}, α i → β i} {i : ι}
+[ha : Inhabited (α i)] [hb : Inhabited (β i)]
+(h : i ∈ mp) : (mp.map f).get! i = f (mp.get! i) := by
+  rcases mp with ⟨xs, h₁⟩
+  simp [get!, get?_map_eq]
+  rw [mem_iff_get?_eq_some] at h
+  obtain ⟨x, h⟩ := h
+  simp [h]
+
+@[simp]
+theorem ofList_nil : ofList (ι := ι) (α := α) [] = ∅ := rfl
+
+@[simp]
+theorem toList_empty : (∅ : DMap ι α).toList = [] := rfl
+
+@[simp]
+theorem ofList_snoc {x : Σ i, α i} {xs} :
+ofList (xs ++ [x]) = (ofList xs).insertProd x := by
+  unfold ofList insertProd
+  ext:1
+  dsimp only
+  generalize ha : [] = acc
+  nth_rewrite 2 [←ha]
+  clear ha
+  induction xs generalizing x acc
+  · simp
+  nm y ys ih
+  dsimp at ih ⊢
+  rw [ih]
+
+@[simp]
+theorem mem'_insert' {x : Σ i, α i} {xs i} :
+mem' i (insert' x xs) ↔ i = x.1 ∨ mem' i xs := by
+  induction xs generalizing x
+  · simp
+  nm y xs ih
+  simp
+  split <;> nm x h₁ <;> clear x
+  · rw [compare_eq_iff_eq] at h₁
+    simp [h₁]
+  · simp
+  · rw [compare_gt_iff_gt, gt_iff_lt] at h₁
+    simp [ih]
+    tauto
+
+@[simp]
+theorem mem_insertProd {x : Σ i, α i} {i} :
+i ∈ mp.insertProd x ↔ i = x.1 ∨ i ∈ mp := by
+  simp [insertProd, mem_def]
+
+-- #check 0 #exit
+
+@[simp]
+theorem mem_ofList {xs : List (Σ i, α i)} {i} :
+i ∈ ofList xs ↔ ∃ x, ⟨i, x⟩ ∈ xs := by
+  induction xs using List.reverseRecOn
+  · simp [mem_def]
+  nm xs x ih
+  simp
+  constructor
+  · rintro (rfl | h)
+    · sorry
+    · sorry
+  · sorry
+
+#check 0 #exit
+
+@[simp]
+theorem mem_range [fin : Fintype ι] {f : (i : ι) → α i} {i : ι} : i ∈ range f := by
+  simp [range]
