AP/Game/Basic.lean
@@ -10,43 +10,70 @@ game.sys.tr a t = some b ↔ a.player = t.1 ∧ ∃ r,
 game.rules t.1 a.state t.2 = some r ∧ b =
 { player := r.1
 , state := r.2
-, hist := t :: a.hist
+, hist := game.updateHist a t
 } := by
-  simp [game.h_sys_tr, GameParams.sys_tr, Option.bind]
-  split
-  · nm x y h₁
-    simp
-    rintro hp p s h₂ rfl
-    simp [h₁] at h₂
-  nm x y z h₁
-  simp
-  intro hp
+  simp only [game.h_sys_tr, GameParams.sys_tr, GameParams.updateHist,
+    Option.bind_eq_bind, Option.bind, Option.dite_none_right_eq_some,
+    updateHist, Prod.exists]
   constructor
-  · rintro ⟨h₂, rfl⟩
+  · rintro ⟨h₁, h₂⟩
+    use h₁
+    split at h₂ <;> simp at h₂
+    nm x y z h₃
     use z.1, z.2
-  · rintro ⟨u, v, h₂, h₃⟩
-    simp [h₁] at h₂
-    subst h₂
-    exact h₃.symm
+    simp [h₁, h₂, h₃]
+  · rintro ⟨h₁, x, y, h₂, rfl⟩
+    use h₁
+    simp [h₁, h₂]
 
 theorem tr_to_iff {a b} {t : T.Trans} :
 game.sys.tr_to a t b ↔ a.player = t.1 ∧ ∃ r,
 game.rules t.1 a.state t.2 = some r ∧ b =
 { player := r.1
 , state := r.2
-, hist := t :: a.hist
+, hist := game.updateHist a t
 } := tr_eq_some_iff
 
-theorem hist_suffix_of_reachable {a b}
-(h : game.sys.Reachable a b) : a.hist <:+ b.hist := by
+@[simp]
+theorem mem_hist_initState {p' p s} : p' ∈ (T.initState p s).hist := by
+  unfold GameParams.initState
+  simp
+  sorry
+
+#check 0 #exit
+
+theorem player_mem_hist_of_valid {a} [hv : game.sys.Valid a] {p} : p ∈ a.hist := by
+  cases hv
+  nm s hs h
+  rcases hs with ⟨hs⟩
+  revert hs
+  induction h <;> clear s <;> intro hs
+  · nm s
+    obtain ⟨p', s', rfl⟩ := @game.h_sys_init_valid _ hs
+    simp
+
+#check 0 #exit
+
+theorem hist_suffix_of_reachable {a} [hv : game.sys.Valid a] {b p}
+(h : game.sys.Reachable a b) : a.hist.get! p <:+ b.hist.get! p := by
+  revert hv
   induction h using System.reachable_ind_right
-  · rfl
+  · intro hv
+    rfl
   clear a b
   nm a b c t h₁ h₂ ih
+  intro hv
+  specialize @ih _
   rw [tr_eq_some_iff] at h₂
-  rcases h₂ with ⟨h₂, ⟨p, c⟩, h₃, rfl⟩
-  simp
-  exact List.suffix_cons_of_suffix ih
+  rcases h₂ with ⟨h₂, ⟨p', c⟩, h₃, rfl⟩
+  simp [Game.updateHist, GameParams.updateHist, h₂]
+  rw [DMap.get!_map_eq_of_pos]
+  rotate_left
+  · 
+  
+  -- exact List.suffix_cons_of_suffix ih
+
+#check 0 #exit
 
 theorem acyclic_gstate {a} : game.sys.Acyclic a := by
   rw [System.acyclic_iff]
